Update proofs

Strata/DL/Lambda/Semantics.lean
@@ -13,18 +13,18 @@ import Strata.DL.Lambda.LState
 
 namespace Lambda
 
-variable {T : LExprParamsT} [DecidableEq T.base.Metadata]
-    [DecidableEq T.base.Identifier] [DecidableEq T.base.IDMeta]
-    [Traceable LExpr.EvalProvenance T.base.Metadata]
+variable {Tbase : LExprParams} [DecidableEq Tbase.Metadata]
+    [DecidableEq Tbase.Identifier] [DecidableEq Tbase.IDMeta]
+    [Traceable LExpr.EvalProvenance Tbase.Metadata]
 
 open Lambda
 
 /--
 A free variable -> expression mapping.
 -/
-abbrev Env (T:LExprParamsT) := T.base.Identifier → Option (LExpr T)
+abbrev Env (Tbase:LExprParams) := Tbase.Identifier → Option (LExpr Tbase.mono)
 
-def Scopes.toFreeVarMap (s:Scopes T.base) : Env T.base.mono :=
+def Scopes.toEnv (s:Scopes Tbase) : Env Tbase :=
   fun t => (s.find? t).map (·.snd)
 
 /--
@@ -41,30 +41,30 @@ assignment to a free variable available.
 metadata must not affect evaluation semantics. Different concrete evaluators
 like LExpr.eval can use different strategy for updating metadata.
 -/
-inductive Step (F:@Factory T.base.mono.base) (rf:Env T.base.mono)
-  : LExpr T.base.mono → LExpr T.base.mono → Prop where
+inductive Step (F:@Factory Tbase) (rf:Env Tbase)
+  : LExpr Tbase.mono → LExpr Tbase.mono → Prop where
 -- A free variable. Stuck if fvar does not exist in FreeVarMap.
 | expand_fvar:
-  ∀ (x:T.base.mono.base.Identifier) (e:LExpr T.base.mono),
+  ∀ (x:Tbase.Identifier) (e:LExpr Tbase.mono),
     rf x = .some e →
-    Step F rf (.fvar _ x ty) e
+    Step F rf (.fvar m x ty) e
 
 -- Beta reduction for lambda; Call-by-value semantics.
 | beta:
-  ∀ (e1 v2 eres:LExpr T.base.mono),
+  ∀ (e1 v2 eres:LExpr Tbase.mono),
     LExpr.isCanonicalValue F v2 →
     eres = LExpr.subst (fun _ => v2) e1 →
     Step F rf (.app m1 (.abs m2 ty e1) v2) eres
 
 -- Call-by-value semantics.
 | reduce_2:
-  ∀ (v1 e2 e2':LExpr T.base.mono),
+  ∀ (v1 e2 e2':LExpr Tbase.mono),
     LExpr.isCanonicalValue F v1 →
     Step F rf e2 e2' →
     Step F rf (.app m v1 e2) (.app m' v1 e2')
 
 | reduce_1:
-  ∀ (e1 e1' e2:LExpr T.base.mono),
+  ∀ (e1 e1' e2:LExpr Tbase.mono),
     Step F rf e1 e1' →
     Step F rf (.app m e1 e2) (.app m' e1' e2)
 
@@ -72,33 +72,33 @@ inductive Step (F:@Factory T.base.mono.base) (rf:Env T.base.mono)
 -- For the reduction order, ite x e1 e2 is interpreted as
 -- 'ite x (λ.e1) (λ.e2)'.
 | ite_reduce_then:
-  ∀ (ethen eelse:LExpr T.base.mono),
+  ∀ (ethen eelse:LExpr Tbase.mono),
     Step F rf (.ite m (.const mc (.boolConst true)) ethen eelse) ethen
 
 | ite_reduce_else:
-  ∀ (ethen eelse:LExpr T.base.mono),
+  ∀ (ethen eelse:LExpr Tbase.mono),
     Step F rf (.ite m (.const mc (.boolConst false)) ethen eelse) eelse
 
 | ite_reduce_cond:
-  ∀ (econd econd' ethen eelse:LExpr T.base.mono),
+  ∀ (econd econd' ethen eelse:LExpr Tbase.mono),
     Step F rf econd econd' →
     Step F rf (.ite m econd ethen eelse) (.ite m' econd' ethen eelse)
 
 -- Equality. Reduce after both operands evaluate to values.
 | eq_reduce:
-  ∀ (e1 e2 eres:LExpr T.base.mono)
+  ∀ (e1 e2 eres:LExpr Tbase.mono)
     (H1:LExpr.isCanonicalValue F e1)
     (H2:LExpr.isCanonicalValue F e2),
     eres = .const mc (.boolConst (LExpr.eql F e1 e2 H1 H2)) →
     Step F rf (.eq m e1 e2) eres
 
 | eq_reduce_lhs:
-  ∀ (e1 e1' e2:LExpr T.base.mono),
+  ∀ (e1 e1' e2:LExpr Tbase.mono),
     Step F rf e1 e1' →
     Step F rf (.eq m e1 e2) (.eq m' e1' e2)
 
 | eq_reduce_rhs:
-  ∀ (v1 e2 e2':LExpr T.base.mono),
+  ∀ (v1 e2 e2':LExpr Tbase.mono),
     LExpr.isCanonicalValue F v1 →
     Step F rf e2 e2' →
     Step F rf (.eq m v1 e2) (.eq m' v1 e2')
@@ -108,7 +108,7 @@ inductive Step (F:@Factory T.base.mono.base) (rf:Env T.base.mono)
 -- the eval_fn constructor below.
 -- This is consistent with what LExpr.eval does (modulo the "inline" flag).
 | expand_fn:
-  ∀ (e callee fnbody new_body:LExpr T.base.mono) args fn,
+  ∀ (e callee fnbody new_body:LExpr Tbase.mono) args fn,
     F.callOfLFunc e = .some (callee,args,fn) →
     args.all (LExpr.isCanonicalValue F) →
     fn.body = .some fnbody →
@@ -119,17 +119,17 @@ inductive Step (F:@Factory T.base.mono.base) (rf:Env T.base.mono)
 -- If LFunc has a concrete evaluator, this can be used to 'jump' to the final
 -- result of the function.
 | eval_fn:
-  ∀ (e callee:LExpr T.base.mono) args fn denotefn,
+  ∀ (e callee:LExpr Tbase.mono) args fn denotefn,
     F.callOfLFunc e = .some (callee,args,fn) →
     args.all (LExpr.isCanonicalValue F) →
     fn.concreteEval = .some denotefn →
     Step F rf e (denotefn (LExpr.mkApp m callee args) args)
 
 
-omit [DecidableEq T.base.Metadata] [DecidableEq T.base.Identifier]
-     [Traceable LExpr.EvalProvenance T.base.Metadata] in
+omit [DecidableEq Tbase.Metadata] [DecidableEq Tbase.Identifier]
+     [Traceable LExpr.EvalProvenance Tbase.Metadata] in
 theorem step_const_stuck:
-  ∀ (F:@Factory T.base) r x e,
+  ∀ (F:@Factory Tbase) r x e,
   ¬ Step F r (.const m x) e := by
   intros
   intro H
@@ -138,8 +138,8 @@ theorem step_const_stuck:
 /--
 Multi-step execution: reflexive transitive closure of single steps.
 -/
-inductive StepStar (F:@Factory T.base) (rf:Env T.base.mono)
-  : LExpr T.base.mono → LExpr T.base.mono → Prop where
+inductive StepStar (F:@Factory Tbase) (rf:Env Tbase)
+  : LExpr Tbase.mono → LExpr Tbase.mono → Prop where
 | refl : StepStar F rf e e
 | step : ∀ e e' e'', Step F rf e e' → StepStar F rf e' e''
         → StepStar F rf e e''
